[helpers] Improve :enable model.
Support enabling functions in the checkpoints, not just the goal.

books/kestrel/helpers/model-enable.lisp
@@ -17,8 +17,54 @@
 (include-book "kestrel/utilities/translate" :dir :system)
 (include-book "kestrel/world-light/defined-fns-in-term" :dir :system)
 (include-book "kestrel/lists-light/firstn-def" :dir :system)
+(include-book "kestrel/typed-lists-light/symbol-listp" :dir :system)
 (include-book "kestrel/utilities/rational-printing" :dir :system)
 
+(local (in-theory (disable mv-nth)))
+
+(local
+ (defthm symbol-listp-of-firstn
+   (implies (symbol-listp syms)
+            (symbol-listp (acl2::firstn n syms)))
+   :hints (("Goal" :in-theory (enable acl2::firstn)))))
+
+(defund acl2::defined-fns-in-terms (terms wrld acc)
+  (declare (xargs :guard (and (pseudo-term-listp terms)
+                              (plist-worldp wrld)
+                              (symbol-listp acc))))
+  (if (endp terms)
+      acc ; todo: think about the order here
+    (acl2::defined-fns-in-terms (rest terms) wrld (union-eq (acl2::defined-fns-in-term (first terms) wrld)
+                                                            acc))))
+
+(defthm symbol-listp-of-defined-fns-in-terms
+  (implies (and (pseudo-term-listp terms)
+                (symbol-listp acc))
+           (symbol-listp (acl2::defined-fns-in-terms terms wrld acc)))
+  :hints (("Goal" :in-theory (enable acl2::defined-fns-in-terms))))
+
+(defund acl2::defined-fns-in-term-lists (term-lists wrld acc)
+  (declare (xargs :guard (and (acl2::pseudo-term-list-listp term-lists)
+                              (plist-worldp wrld)
+                              (symbol-listp acc))))
+  (if (endp term-lists)
+      acc
+    (acl2::defined-fns-in-term-lists (rest term-lists) wrld (acl2::defined-fns-in-terms (first term-lists) wrld acc))))
+
+(defthm symbol-listp-of-defined-fns-in-term-lists
+  (implies (and (acl2::pseudo-term-list-listp term-lists)
+                (symbol-listp acc))
+           (symbol-listp (acl2::defined-fns-in-term-lists term-lists wrld acc)))
+  :hints (("Goal" :in-theory (enable acl2::defined-fns-in-term-lists))))
+
+;move
+(local
+ (defthm rationalp-of-mv-nth-0-of-read-run-time
+  (rationalp (mv-nth 0 (read-run-time state)))
+  :rule-classes :type-prescription
+  :hints (("Goal" :in-theory (enable read-run-time)))))
+
+;; todo: support enabling more than one thing in a single rec
 (defun make-enable-recs-aux (names num)
   (declare (xargs :guard (and (symbol-listp names)
                               (posp num))))
@@ -41,14 +87,17 @@
 ;; TODO: Don't even make recs for things that are enabled (in the theory, or by the current hints)?
 ;; TODO: Put in macro-aliases, like append, when possible.  What if there are multiple macro-aliases for a function?  Prefer ones that appear in the untranslated formula?
 ;; Returns (mv erp recs state), where recs is a list of recs, which should contain no duplicates.
-(defun make-enable-recs (formula ; an untranslated term
+(defun make-enable-recs (translated-theorem-body
+                         checkpoint-clauses
                          num-recs
                          print
                          state)
-  (declare (xargs :guard (and (natp num-recs)
+  (declare (xargs :guard (and (pseudo-termp translated-theorem-body)
+                              (acl2::pseudo-term-list-listp checkpoint-clauses)
+                              (natp num-recs)
                               (acl2::print-levelp print))
                   :stobjs state
-                  :mode :program ; because of acl2::translate-term
+;                  :mode :program ; because of acl2::translate-term
                   ))
   (b* ((wrld (w state))
        (- (and (acl2::print-level-at-least-tp print)
@@ -56,18 +105,37 @@
                    num-recs)))
        (print-timep (acl2::print-level-at-least-tp print))
        ((mv start-time state) (if print-timep (acl2::get-real-time state) (mv 0 state)))
-       (translated-formula (acl2::translate-term formula 'make-enable-recs wrld))
-       (fns-to-try-enabling (set-difference-eq (acl2::defined-fns-in-term translated-formula wrld)
+       ; (translated-formula (acl2::translate-term formula 'make-enable-recs wrld))
+       (fns-in-goal (set-difference-eq (acl2::defined-fns-in-term translated-theorem-body wrld)
                                                ;; Don't bother wasting time with trying to enable implies
                                                ;; (I suppose we could try it if implies is disabled):
-                                               '(implies)))
-       (recs-to-return ;; todo: how to choose when we can't return them all?:
-        (acl2::firstn num-recs (make-enable-recs-aux fns-to-try-enabling 1)))
+                                       '(implies)))
+       (fns-in-checkpoints (acl2::defined-fns-in-term-lists checkpoint-clauses wrld nil))
+       (fns-only-in-checkpoints (set-difference-eq fns-in-checkpoints fns-in-goal))
+       ;; we'll try the ones in the goal first (todo: do a more sophisticated ranking?):
+       ;; todo: prefer ones defined in the current book?  more complex ones?
+       ;; todo: make a rec that enables all (sensible functions?)
+       ;; todo: remove any functions already enabled, at least in the goal hint?
+       ;; todo: try all defined functions in the conclusion
+       ;; todo: try all defined functions
+       ;; the order here matters (todo: what order to choose?)
+       (fns-to-try-enabling (append fns-in-goal fns-only-in-checkpoints))
+       (fns-to-try-enabling (acl2::firstn num-recs fns-to-try-enabling))
+       (fns-beyond-the-limit (nthcdr num-recs fns-to-try-enabling))
+       (- (and fns-beyond-the-limit
+               (cw "Suppressing ~x0 enable recs (beyond num-recs): ~X12.~%" (len fns-beyond-the-limit) fns-beyond-the-limit nil)))
+       (recs (make-enable-recs-aux fns-to-try-enabling 1))
+       ;; Compute elapsed time:
        ((mv done-time state) (if print-timep (acl2::get-real-time state) (mv 0 state)))
-       (- (and print-timep (prog2$ (acl2::print-to-hundredths (- done-time start-time))
+       (time-diff (- done-time start-time))
+       (time-diff (if (< time-diff 0)
+                      (prog2$ (cw "Warning: negative time reported: ~x0.~%")
+                              0)
+                    time-diff))
+       (- (and print-timep (prog2$ (acl2::print-to-hundredths time-diff)
                                    (cw "s~%") ; s = seconds
                                    ))))
-    (mv nil recs-to-return state)))
+    (mv nil recs state)))
 
 ;; (local
 ;;  (defthm recommendation-listp-of-make-enable-recs
